LambdaGraph/Lemmas.lean
@@ -1,17 +1,37 @@
 import LambdaGraph.Basic
 
+@[simp]
+theorem not_closed_var {p : Env} {n : Nat} : ¬(Expr.var n).Closed p :=
+  fun h => h n .var
+
+theorem fn_closed_iff {p : Env} {m : Nat} :
+    (Expr.fn m).Closed p ↔ ∀ n ≠ m, (_ : m < p.size) → ¬p.fn[m].Free p n := by
+  constructor
+  · intro hc n hn _
+    intro hne
+    solve_by_elim
+  · intro hf n hn
+    cases hn with
+    | fn _ _ hne hn =>
+      solve_by_elim
+
+@[simp]
 theorem app_closed_iff {p : Env} {f e : Expr} :
     (f.app e).Closed p ↔ f.Closed p ∧ e.Closed p := by
   constructor
   · intro h
-    constructor <;> solve_by_elim [Free.appL, Free.appR]
+    constructor <;> solve_by_elim [Expr.Free.appL, Expr.Free.appR]
   · rintro ⟨hf, he⟩ n (- | -) <;> solve_by_elim
 
+@[simp]
+theorem bool_closed (p : Env) (b : Bool) : (Expr.bool b).Closed p := nofun
+
+@[simp]
 theorem cond_closed_iff {p : Env} {c et ef : Expr} :
     (c.cond et ef).Closed p ↔ c.Closed p ∧ et.Closed p ∧ ef.Closed p := by
   constructor
   · intro h
-    and_intros <;> solve_by_elim [Free.condC, Free.condT, Free.condF]
+    and_intros <;> solve_by_elim [Expr.Free.condC, Expr.Free.condT, Expr.Free.condF]
   · rintro ⟨hc, het, hef⟩ n (- | - | -) <;> solve_by_elim
 
 theorem value_types_cn {p : Env} {v : Expr} {t : Ty} (h : p ⊢ v : t.cn) :
@@ -24,11 +44,491 @@ theorem value_types_bool {p : Env} {v : Expr} (h : p ⊢ v : .bool) :
   | .fn n => nomatch h
   | .bool b => by simp
 
-theorem progress (p : Program) (t : Ty) (ht : ⊢ p : t) (hc : p.Closed) :
+theorem size_le_of_step {p p' : Program} (h : p ⇒ p') : p.size ≤ p'.size := by
+  induction h with simp [*, Env.subst, Program.subst]
+
+theorem lt_size_of_step {p p' : Program} {n : Nat} (hn : n < p.size)
+    (h : p ⇒ p') : n < p'.size := Nat.lt_of_lt_of_le hn (size_le_of_step h)
+
+theorem fn_eq_of_step {p p' : Program} {n : Nat} (hn : n < p.size) (h : p ⇒ p')
+    : p.fn[n] = p'.fn[n]'(lt_size_of_step hn h) := by
+  induction h with simp [*, Env.subst, Program.subst]
+
+theorem ty_eq_of_step {p p' : Program} {n : Nat} (hn : n < p.size) (h : p ⇒ p')
+    : p.ty[n] = p'.ty[n]'(lt_size_of_step hn h) := by
+  induction h with simp [*, Env.subst, Program.subst]
+
+theorem types_of_step {p p' : Program} {e : Expr} {t : Ty} (ht : p.toEnv ⊢ e : t)
+    (hs : p ⇒ p') : p'.toEnv ⊢ e : t := by
+  induction ht with
+    (try rw [ty_eq_of_step ‹_› hs]) <;> constructor <;> assumption
+
+theorem env_subst_size_le {p : Env} {v : Expr} {n : Nat} {map : LabelMap p} :
+    p.size ≤ (p.subst map n v).size := by
+  simp [Env.subst]
+
+theorem lt_subst_size {p : Env} (v : Expr) {n : Nat} (map : LabelMap p)
+    (hn : n < p.size) : n < (p.subst map n v).size :=
+  Nat.lt_of_lt_of_le hn env_subst_size_le
+
+theorem subst_fn_eq {p : Env} (v : Expr) {m n : Nat} (map : LabelMap p)
+    (hn : m < p.size) :
+    (p.subst map n v).fn[m]'(lt_subst_size v map hn) = p.fn[m] := by
+  simp [hn, Env.subst]
+
+theorem subst_ty_eq {p : Env} (v : Expr) {m n : Nat} (map : LabelMap p)
+    (hn : m < p.size) :
+    (p.subst map n v).ty[m]'(lt_subst_size v map hn) = p.ty[m] := by
+  simp [hn, Env.subst]
+
+theorem expr_types_in_subst {p : Env} {e : Expr} (v : Expr) {t : Ty} (n : Nat)
+    (map : LabelMap p) (ht : p ⊢ e : t) :
+    p.subst map n v ⊢ e : t := by
+  induction ht with try constructor <;> assumption
+  | var m hm =>
+    rw [← subst_ty_eq v map hm]
+    constructor
+  | fn m hm =>
+    rw [← subst_ty_eq v map hm]
+    constructor
+
+theorem Depends.lt {p : Env} {m n : Nat} : Depends p m n → m < p.size
+  | free _ _ hm _ _ => hm
+  | step _ _ _ hm _ _ _ => hm
+
+theorem depends_self {p : Env} {n : Nat} :
+    (h : Depends p n n) → ∃ m ≠ n, (p.fn[n]'h.lt).Free p m
+  | .free _ _ _ hne _ => nomatch hne
+  | .step _ k _ _ hne hf _ => ⟨k, hne, hf⟩
+
+structure LabelMap.ValidNew {p : Env} (map : LabelMap p) {i : Nat}
+    (h : i < p.size) : Prop where
+  fwd_ge : p.size ≤ map.fwd[i]
+  fwd_lt : map.fwd[i] < p.size + map.inv.size
+  inv_fwd_sub : map.inv[map.fwd[i] - p.size] = i
+
+structure LabelMap.Valid {p : Env} (map : LabelMap p) (n : Nat) : Prop where
+  lt : n < p.size
+  not_depends : ∀ {i} (h : i < p.size), ¬Depends p i n → map.fwd[i] = i
+  depends : ∀ {i} (h : i < p.size), Depends p i n → map.ValidNew h
+
+theorem LabelMap.Valid.eq_or_new {p : Env} {map : LabelMap p} {n : Nat}
+    (hmap : map.Valid n) {i : Nat} (hi : i < p.size) :
+    map.fwd[i] = i ∨ map.ValidNew hi := by
+  by_cases h : Depends p i n
+  · right
+    exact hmap.depends hi h
+  · left
+    exact hmap.not_depends hi h
+
+theorem LabelMap.Valid.fwd_lt {p : Env} {map : LabelMap p} {n : Nat}
+    (hmap : map.Valid n) {i : Nat} (hi : i < p.size) :
+    map.fwd[i] < p.size + map.inv.size := by
+  rcases hmap.eq_or_new hi with h | h
+  · rw [h]
+    omega
+  · exact h.fwd_lt
+
+theorem labelMap_valid (p : Env) {n : Nat} (hn : n < p.size) :
+    (p.labelMap n).Valid n where
+  lt := hn
+  not_depends := by
+    intro i hi h
+    unfold Env.labelMap
+    simp [aux_le_not_depends hi (Nat.zero_le i) h]
+  depends := by
+    intro i hi h
+    unfold Env.labelMap
+    exact aux_le_depends hi (Nat.zero_le i) h
+where
+  aux_gt_map {i j map inv} (hi : i < p.size) (hj : i < j) :
+      (Env.labelMap.aux p n j map inv).1[i] = map[i] := by
+    have (eq := hd) d := p.size - j
+    induction d generalizing j map inv with unfold Env.labelMap.aux
+    | zero => simp [show ¬j < p.size by omega]
+    | succ d ih =>
+      split
+      · split
+        · have : map[i] = (map.set j (p.size + inv.size) ‹j < p.size›)[i] := by
+            simp [show j ≠ i by omega]
+          rw [this]
+          apply ih <;> omega
+        · apply ih <;> omega
+      · simp
+  aux_inv_size_ge {j map inv} :
+      inv.size ≤ (Env.labelMap.aux p n j map inv).2.size := by
+    have (eq := hd) d := p.size - j
+    induction d generalizing j map inv with unfold Env.labelMap.aux
+    | zero => simp [show ¬j < p.size by omega]
+    | succ d ih =>
+      have hj : j < p.size := by omega
+      simp only [hj, ↓reduceDIte, ge_iff_le]
+      split
+      · have hle : inv.size ≤ (inv.push ⟨j, hj⟩).size := by simp
+        apply Nat.le_trans hle
+        apply ih
+        omega
+      · apply ih
+        omega
+  aux_gt_inv {i j k map inv} (hk : k < inv.size)
+      (hk' : k < (Env.labelMap.aux p n j map inv).2.size) :
+      (Env.labelMap.aux p n j map inv).2[k] = inv[k] := by
+    have (eq := hd) d := p.size - j
+    induction d generalizing j map inv with unfold Env.labelMap.aux
+    | zero => simp [show ¬j < p.size by omega]
+    | succ d ih =>
+      have hj : j < p.size := by omega
+      simp [hj]
+      split
+      · have : inv[k] = (inv.push ⟨j, hj⟩)[k]'(by rw [Array.size_push]; omega) :=
+          Eq.symm (Array.getElem_push_lt hk)
+        rw [this]
+        apply ih
+        omega
+      · apply ih
+        omega
+  aux_le_not_depends {i j map inv} (hi : i < p.size) (hj : j ≤ i)
+      (h : ¬Depends p i n) :
+      (Env.labelMap.aux p n j map inv).1[i] = map[i] := by
+    have (eq := hd) d := i - j
+    induction d generalizing j map inv with unfold Env.labelMap.aux
+    | zero =>
+      simp only [*, show j = i by omega]
+      apply aux_gt_map
+      simp
+    | succ d ih =>
+      have hj' := Nat.lt_of_le_of_lt hj hi
+      simp only [hj', ↓reduceDIte]
+      split
+      · have : map[i] = (map.set j (p.size + inv.size) hj')[i] := by
+          simp [show j ≠ i by omega]
+        rw [this]
+        apply ih <;> omega
+      · apply ih <;> omega
+  aux_le_depends {i j map inv} (hi : i < p.size) (hj : j ≤ i)
+      (h : Depends p i n) :
+      let (map', inv') := Env.labelMap.aux p n j map inv
+      LabelMap.ValidNew ⟨map', inv'⟩ hi := by
+    have (eq := hd) d := i - j
+    induction d generalizing j map inv with unfold Env.labelMap.aux
+    | zero =>
+      simp [*, show j = i by omega]
+      refine ⟨?_, ?_, ?_⟩
+      · simp [aux_gt_map]
+      · have hlt : inv.size < (inv.push ⟨i, hi⟩).size := by simp
+        simp only [Nat.lt_add_one, aux_gt_map, Vector.getElem_set_self,
+          Nat.add_lt_add_iff_left]
+        apply Nat.lt_of_lt_of_le hlt
+        simp only [aux_inv_size_ge]
+      · simp only [Nat.lt_add_one, aux_gt_map, Vector.getElem_set_self,
+          Nat.add_sub_cancel_left]
+        have : i = (inv.push ⟨i, hi⟩)[inv.size] := by simp
+        conv => rhs; rw [this]
+        rw [aux_gt_inv]
+        exact 0 -- what?
+    | succ d ih =>
+      have hj' : j < p.size := by omega
+      simp [hj']
+      split <;> apply ih <;> omega
+
+theorem subst_ty_map_eq {p : Env} {v : Expr} {m n : Nat} {map : LabelMap p}
+    (hm : m < p.size) (hmap : map.Valid n) :
+    (p.subst map n v).ty[map.fwd[m]]'(hmap.fwd_lt hm) = p.ty[m] := by
+  rcases hmap.eq_or_new hm with h | ⟨hle, hlt, hinv⟩
+  · simp [h, hm, Env.subst]
+  · simp [*, Env.subst]
+
+theorem expr_subst_types {p : Env} {e v : Expr} {t : Ty} {n : Nat}
+    {map : LabelMap p} (hmap : map.Valid n) (ht : p ⊢ e : t)
+    (htv : p ⊢ v : p.ty[n]'hmap.lt) :
+    p.subst map n v ⊢ e.subst map n v : t := by
+  induction ht with try constructor <;> assumption
+  | var m hm =>
+    by_cases hnm : n = m
+    · subst m
+      simp [Expr.subst]
+      exact expr_types_in_subst _ _ _ htv
+    · have hm' : m < map.fwd.size := hm
+      simp [hnm, hm', Expr.subst]
+      rw [← subst_ty_map_eq hm hmap]
+      constructor
+  | fn m hm =>
+    simp only [Expr.subst, hm, getElem?_pos, Option.getD_some]
+    rw [← subst_ty_map_eq hm hmap]
+    constructor
+
+theorem subst_types {p : Env} {e v : Expr} {t : Ty} {n : Nat} (hn : n < p.size)
+    (ht : ⊢ ⟨p, e⟩ : t) (htv : p ⊢ v : p.ty[n]) :
+    ⊢ Program.subst ⟨p, e⟩ n v : t := by
+  obtain ⟨htp, ht⟩ := ht
+  dsimp only at *
+  constructor
+  · intro m hm
+    simp [Env.subst, Program.subst]
+    by_cases hm' : m < p.size
+    · simp [hm']
+      exact expr_types_in_subst _ _ _ (htp _)
+    · simp at hm'
+      simp [hm']
+      exact expr_subst_types (labelMap_valid _ hn) (htp _) htv
+  · exact expr_subst_types (labelMap_valid _ hn) ht htv
+
+inductive Expr.ValidRefs (p : Env) : Expr → Prop where
+  | var (n : Nat) : n < p.size → (Expr.var n).ValidRefs p
+  | fn (n : Nat) : n < p.size → (Expr.fn n).ValidRefs p
+  | app (f e : Expr) : f.ValidRefs p → e.ValidRefs p → (f.app e).ValidRefs p
+  | bool (b : Bool) : (Expr.bool b).ValidRefs p
+  | cond (c et ef : Expr) : c.ValidRefs p → et.ValidRefs p → ef.ValidRefs p →
+    (c.cond et ef).ValidRefs p
+
+theorem Expr.Types.validRefs {p : Env} {e : Expr} {t : Ty} (ht : p ⊢ e : t) :
+    e.ValidRefs p := by
+  induction ht with constructor <;> assumption
+
+def Env.ValidRefs (p : Env) : Prop :=
+  ∀ {i} (_ : i < p.size), p.fn[i].ValidRefs p
+
+theorem Env.Types.validRefs {p : Env} (ht : ⊢ p) : p.ValidRefs :=
+  fun hi => (ht hi).validRefs
+
+theorem lt_size_of_free {p : Env} {e : Expr} {n : Nat} (hp : p.ValidRefs)
+    (he : e.ValidRefs p) (hf : e.Free p n) : n < p.size := by
+  induction hf with cases he <;> apply_rules
+
+theorem subst_eq_var {p : Env} {e v : Expr} {m n : Nat}
+    {map : LabelMap p} (he : e.ValidRefs p) (hc : v.Closed p)
+    (h : e.subst map n v = .var m) :
+    ∃ (i : Fin p.size), m = map.fwd[i] ∧ e = .var i := by
+  cases e with simp only [Expr.subst] at h <;> try contradiction
+  | var k =>
+    have .var _ hk := he
+    by_cases hnk : n = k
+    · simp only [hnk, ↓reduceIte] at h
+      subst v
+      exfalso
+      exact hc m .var
+    · exists ⟨k, hk⟩
+      simpa [hnk, hk, eq_comm] using h
+
+theorem subst_ne_subst_var {p : Env} {e v : Expr} {n : Nat}
+    {map : LabelMap p} (hmap : map.Valid n) (hv : v.Value) :
+    e.subst map n v ≠ .var n := by
+  cases e with simp only [Expr.subst] <;> try intro; contradiction
+  | var m =>
+    split
+    · intro rfl
+      nomatch hv
+    · by_cases hm : m < p.size
+      · rcases hmap.eq_or_new hm with hm | ⟨hle, hlt, hinv⟩
+        · simp [*, Ne.symm]
+        · simp [hm]
+          intro h
+          rw [h] at hle
+          have := hmap.lt
+          omega
+      · simp [*, Ne.symm]
+
+theorem subst_eq_fn {p : Env} {e v : Expr} {m n : Nat} {map : LabelMap p}
+    (he : e.ValidRefs p) (h : e.subst map n v = .fn m) :
+    e = .var n ∨ ∃ i : Fin p.size, m = map.fwd[i] ∧ e = .fn i := by
+  cases e with simp only [Expr.subst] at h <;> try contradiction
+  | var k =>
+    split at h
+    · simp [*]
+    · simp at h
+  | fn k =>
+    right
+    have .fn _ hk := he
+    exists ⟨k, hk⟩
+    simpa [hk, eq_comm] using h
+
+theorem subst_eq_app {p : Env} {e e₁ e₂ v : Expr} {n : Nat} {map : LabelMap p}
+    (hv : v.Value) (h : e.subst map n v = e₁.app e₂) :
+    ∃ e₁' e₂' : Expr, e = e₁'.app e₂' := by
+  cases e with try solve | simp [Expr.subst] at h
+  | var m =>
+    by_cases hnm : n = m
+    · simp only [Expr.subst, hnm, ↓reduceIte] at h
+      subst v
+      nomatch hv
+    · simp [hnm, Expr.subst] at h
+  | app e₁' e₂' =>
+    simp only [Expr.subst, Expr.app.injEq] at h
+    exists e₁', e₂'
+
+theorem subst_eq_cond {p : Env} {e c et ef v : Expr} {n : Nat} {map : LabelMap p}
+    (hv : v.Value) (h : e.subst map n v = c.cond et ef) :
+    ∃ c' et' ef' : Expr, e = c'.cond et' ef' := by
+  cases e with try solve | simp [Expr.subst] at h
+  | var m =>
+    by_cases hnm : n = m
+    · simp only [Expr.subst, hnm, ↓reduceIte] at h
+      subst v
+      nomatch hv
+    · simp [hnm, Expr.subst] at h
+  | cond c' et' ef' =>
+    simp only [Expr.subst, Expr.cond.injEq] at h
+    exists c', et', ef'
+
+theorem free_of_free_in_subst {p : Env} {e v : Expr} {m n : Nat}
+    {map : LabelMap p} (hp : p.ValidRefs) (he : e.ValidRefs p)
+    (hf : e.Free (p.subst map n v) m) : e.Free p m := by
+  generalize hp' : p.subst map n v = p' at hf
+  open Expr.Free in
+  induction hf with
+    try solve | cases he; solve_by_elim [appL, appR, condC, condT, condF]
+  | fn k hk' hne hf ih =>
+    have .fn _ hk := he
+    constructor
+    · exact hne
+    · subst p'
+      rw [subst_fn_eq _ _ hk] at ih
+      exact ih (hp hk)
+
+theorem not_free_in_subst {p : Env} {e v : Expr} {n : Nat} {map : LabelMap p}
+    (hmap : map.Valid n) (hp : p.ValidRefs) (he : e.ValidRefs p)
+    (hv : v.ValidRefs p) (hc : v.Closed p) (hvv : v.Value) :
+    ¬(e.subst map n v).Free (p.subst map n v) n := by
+  intro hf
+  generalize hp' : p.subst map n v = p', he' : e.subst map n v = e' at hf
+  induction hf generalizing e with
+  | var => exact subst_ne_subst_var hmap hvv he'
+  | fn m hm' hne hf ih =>
+    subst p'
+    rcases subst_eq_fn he he' with rfl | ⟨⟨i, hi⟩, rfl, rfl⟩
+    · simp only [Expr.subst, ↓reduceIte] at he'
+      subst v
+      have .fn _ hm := hv
+      rw [subst_fn_eq _ _ hm] at hf
+      replace hf := free_of_free_in_subst hp (hp hm) hf
+      exact hc n (.fn _ _ hne hf)
+    · by_cases hd : Depends p i n
+      · obtain ⟨hle, hlt, hinv⟩ := hmap.depends hi hd
+        exact ih (hp hi) (by simp [*, Env.subst])
+      · have hi' := hmap.not_depends hi hd
+        simp only [Fin.getElem_fin, hi', subst_fn_eq _ _ hi] at hf
+        simp only [Fin.getElem_fin, hi', ne_eq] at hne
+        replace hf := free_of_free_in_subst hp (hp hi) hf
+        exact hd (.free _ _ _ hne hf)
+  | appL f e'' hf ih =>
+    obtain ⟨f', e''', rfl, rfl⟩ := subst_eq_app hvv he'
+    simp only [Expr.subst] at he'
+    obtain ⟨rfl, rfl⟩ := he'
+    replace .app _ _ hf he := he
+    exact ih hf rfl
+  | appR f e'' hf ih =>
+    obtain ⟨f', e''', rfl, rfl⟩ := subst_eq_app hvv he'
+    simp only [Expr.subst] at he'
+    obtain ⟨rfl, rfl⟩ := he'
+    replace .app _ _ hf he := he
+    exact ih he rfl
+  | condC c et ef hf ih =>
+    obtain ⟨c', et', ef', rfl, rfl, rfl⟩ := subst_eq_cond hvv he'
+    simp only [Expr.subst] at he'
+    obtain ⟨rfl, rfl, rfl⟩ := he'
+    have .cond _ _ _ hc het hef := he
+    exact ih hc rfl
+  | condT c et ef hf ih =>
+    obtain ⟨c', et', ef', rfl, rfl, rfl⟩ := subst_eq_cond hvv he'
+    simp only [Expr.subst] at he'
+    obtain ⟨rfl, rfl, rfl⟩ := he'
+    have .cond _ _ _ hc het hef := he
+    exact ih het rfl
+  | condF c et ef hf ih =>
+    obtain ⟨c', et', ef', rfl, rfl, rfl⟩ := subst_eq_cond hvv he'
+    simp only [Expr.subst] at he'
+    obtain ⟨rfl, rfl, rfl⟩ := he'
+    have .cond _ _ _ hc het hef := he
+    exact ih hef rfl
+
+theorem eq_map_of_free_in_subst {p : Env} {e v : Expr} {m n : Nat}
+    {map : LabelMap p} (hmap : map.Valid n) (hp : p.ValidRefs)
+    (he : e.ValidRefs p) (hv : v.ValidRefs p) (hc : v.Closed p)
+    (hvv : v.Value) (hf : (e.subst map n v).Free (p.subst map n v) m) :
+    ∃ (i : Fin p.size), m = map.fwd[i] ∧ e.Free p i := by
+  generalize hp' : p.subst map n v = p', he' : e.subst map n v = e' at hf
+  induction hf generalizing e with
+  | var =>
+    obtain ⟨⟨i, hi⟩, rfl, rfl⟩ := subst_eq_var he hc he'
+    exists ⟨i, hi⟩
+    simp [Expr.Free.var]
+  | fn k hk' hne hf ih =>
+    subst p'
+    rcases subst_eq_fn he he' with rfl | ⟨⟨i, hi⟩, rfl, rfl⟩
+    · simp only [Expr.subst, ↓reduceIte] at he'
+      subst v
+      have .fn _ hk := hv
+      rw [subst_fn_eq _ _ hk] at hf
+      replace hf := free_of_free_in_subst hp (hp hk) hf
+      exfalso
+      exact hc m (.fn _ _ hne hf)
+    · by_cases hd : Depends p i n
+      · obtain ⟨hle, hlt, hinv⟩ := hmap.depends hi hd
+        obtain ⟨j, rfl, hj⟩ := ih (hp hi) (by simp [*, Env.subst])
+        have hij : j ≠ i := by
+          intro rfl
+          contradiction
+        exact ⟨j, rfl, .fn _ hi hij hj⟩
+      · obtain hi' := hmap.not_depends hi hd
+        simp only [Fin.getElem_fin, hi', subst_fn_eq v map hi] at hf
+        replace hf := free_of_free_in_subst hp (hp hi) hf
+        simp [hi'] at hne
+        have hm : ¬Depends p m n := fun h => hd (.step _ _ _ hi hne hf h)
+        have hlt := lt_size_of_free hp (hp hi) hf
+        have hm' := hmap.not_depends hlt hm
+        refine ⟨⟨m, hlt⟩, by simp [hm'], .fn _ hi hne hf⟩
+  | appL f e'' hf ih =>
+    obtain ⟨f', e''', rfl, rfl⟩ := subst_eq_app hvv he'
+    simp only [Expr.subst] at he'
+    obtain ⟨rfl, rfl⟩ := he'
+    replace .app _ _ hf he := he
+    obtain ⟨i, rfl, hf'⟩ := ih hf rfl
+    exact ⟨i, rfl, .appL _ _ hf'⟩
+  | appR f e'' hf ih =>
+    obtain ⟨f', e''', rfl, rfl⟩ := subst_eq_app hvv he'
+    simp only [Expr.subst] at he'
+    obtain ⟨rfl, rfl⟩ := he'
+    replace .app _ _ hf he := he
+    obtain ⟨i, rfl, hf'⟩ := ih he rfl
+    exact ⟨i, rfl, .appR _ _ hf'⟩
+  | condC c et ef hf ih =>
+    obtain ⟨c', et', ef', rfl, rfl, rfl⟩ := subst_eq_cond hvv he'
+    simp only [Expr.subst] at he'
+    obtain ⟨rfl, rfl, rfl⟩ := he'
+    have .cond _ _ _ hc het hef := he
+    obtain ⟨i, rfl, hf'⟩ := ih hc rfl
+    exact ⟨i, rfl, .condC _ _ _ hf'⟩
+  | condT c et ef hf ih =>
+    obtain ⟨c', et', ef', rfl, rfl, rfl⟩ := subst_eq_cond hvv he'
+    simp only [Expr.subst] at he'
+    obtain ⟨rfl, rfl, rfl⟩ := he'
+    have .cond _ _ _ hc het hef := he
+    obtain ⟨i, rfl, hf'⟩ := ih het rfl
+    exact ⟨i, rfl, .condT _ _ _ hf'⟩
+  | condF c et ef hf ih =>
+    obtain ⟨c', et', ef', rfl, rfl, rfl⟩ := subst_eq_cond hvv he'
+    simp only [Expr.subst] at he'
+    obtain ⟨rfl, rfl, rfl⟩ := he'
+    have .cond _ _ _ hc het hef := he
+    obtain ⟨i, rfl, hf'⟩ := ih hef rfl
+    exact ⟨i, rfl, .condF _ _ _ hf'⟩
+
+theorem closed_of_step {p p' : Program} {e : Expr} (hp : p.ValidRefs)
+    (he : e.ValidRefs p.toEnv) (hc : e.Closed p.toEnv) (hs : p ⇒ p') :
+    e.Closed p'.toEnv := by
+  intro m hf
+  apply hc m
+  induction hs with
+    dsimp only at * <;> apply_rules
+  | app =>
+    dsimp only [Program.subst] at *
+    exact free_of_free_in_subst hp he hf
+
+theorem progress {p : Program} {t : Ty} (ht : ⊢ p : t) (hc : p.Closed) :
     p.expr.Value ∨ ∃ p', p ⇒ p' := by
   obtain ⟨p, e⟩ := p
   obtain ⟨htp, hte⟩ := ht
-  simp only [Program.Closed] at *
+  simp only at *
   induction hte with
   | var n hn => exfalso; exact hc n .var
   | fn n hn => left; constructor
@@ -38,11 +538,8 @@ theorem progress (p : Program) (t : Ty) (ht : ⊢ p : t) (hc : p.Closed) :
     rcases ihf hcf with hvf | ⟨p', hp⟩
     · rcases ihe hce with hve | ⟨p', hp⟩
       · obtain ⟨n, rfl⟩ := value_types_cn htf hvf
-        constructor
-        constructor
-        · cases htf
-          assumption
-        · exact hve
+        cases htf
+        solve_by_elim [Exists.intro]
       · exact ⟨_, Step.appR _ _ _ _ _ hvf hp⟩
     · exact ⟨_, Step.appL _ _ _ _ _ hp⟩
   | bool b => left; constructor
@@ -52,3 +549,103 @@ theorem progress (p : Program) (t : Ty) (ht : ⊢ p : t) (hc : p.Closed) :
     rcases ihc hcc with hvc | ⟨p', hp⟩
     · rcases value_types_bool htc hvc with ⟨_ | _, rfl⟩ <;> repeat constructor
     · exact ⟨_, Step.condC _ _ _ _ _ _ hp⟩
+
+theorem preservation_types {p p' : Program} {t : Ty} (ht : ⊢ p : t)
+  (hs : p ⇒ p') : ⊢ p' : t := by
+  obtain ⟨htp, ht⟩ := ht
+  induction hs generalizing t with
+  | app p n e h hv =>
+    have .app _ _ t htf hte := ht
+    cases htf
+    solve_by_elim [subst_types]
+  | appL p p' f f' e hs ih =>
+    have .app _ _ t htf hte := ht
+    obtain ⟨htp', htf'⟩ := ih htp htf
+    constructor
+    · exact htp'
+    · dsimp only at *
+      constructor
+      · exact htf'
+      · exact types_of_step hte hs
+  | appR p p' f e e' hvf hs ih =>
+    have .app _ _ t htf hte := ht
+    obtain ⟨htp', hte'⟩ := ih htp hte
+    constructor
+    · exact htp'
+    · dsimp only at *
+      constructor
+      · exact types_of_step htf hs
+      · exact hte'
+  | condT p et ef => cases ht; constructor <;> assumption
+  | condF p et ef => cases ht; constructor <;> assumption
+  | condC p p' c c' et ef hs ih =>
+    have .cond _ _ _ _ htc htet htef := ht
+    obtain ⟨htp', htc'⟩ := ih htp htc
+    constructor
+    · exact htp'
+    · dsimp only at *
+      constructor
+      · exact htc'
+      · exact types_of_step htet hs
+      · exact types_of_step htef hs
+
+theorem preservation_closed {p p' : Program} {t : Ty} (ht : ⊢ p : t)
+    (hc : p.Closed) (hs : p ⇒ p') : p'.Closed := by
+  obtain ⟨htp, ht⟩ := ht
+  induction hs generalizing t with
+  | app p n e hn hve =>
+    intro m hm
+    obtain ⟨hcf, hce⟩ := app_closed_iff.mp hc
+    have .app _ _ t' htf hte := ht
+    have hmap : (p.labelMap n).Valid n := labelMap_valid _ hn
+    have hp : p.ValidRefs := htp.validRefs
+    have hfn := hp hn
+    have he := hte.validRefs
+    have hne : n ≠ m := by
+      intro rfl
+      simp [Program.subst, Program.Free] at hm
+      exact not_free_in_subst hmap hp hfn he hce hve hm
+    obtain ⟨⟨i, hi⟩, rfl, hf⟩ :=
+      eq_map_of_free_in_subst hmap hp hfn he hce hve hm
+    simp only [Fin.getElem_fin] at hne
+    simp only at hf
+    have hd : ¬Depends p n n := by
+      intro hd
+      obtain ⟨m, hm, hf⟩ := depends_self hd
+      exact hcf m (.fn _ _ hm hf)
+    have hne : i ≠ n := by
+      intro rfl
+      simp [hmap.not_depends hi hd] at hne
+    exact hcf i (.fn _ hn hne hf)
+  | appL p p' f f' e hs ih =>
+    obtain ⟨hcf, hce⟩ := app_closed_iff.mp hc
+    apply app_closed_iff.mpr
+    have .app _ _ t' htf hte := ht
+    dsimp only at *
+    constructor
+    · exact ih hcf htp htf
+    · exact closed_of_step htp.validRefs hte.validRefs hce hs
+  | appR p p' f e e' hvf hs ih =>
+    obtain ⟨hcf, hce⟩ := app_closed_iff.mp hc
+    apply app_closed_iff.mpr
+    have .app _ _ t' htf hte := ht
+    dsimp only at *
+    constructor
+    · exact closed_of_step htp.validRefs htf.validRefs hcf hs
+    · exact ih hce htp hte
+  | condT p et ef =>
+    obtain ⟨-, hcet, -⟩ := cond_closed_iff.mp hc
+    exact hcet
+  | condF p et ef =>
+    obtain ⟨-, -, hcef⟩ := cond_closed_iff.mp hc
+    exact hcef
+  | condC p p' c c' et ef hs ih =>
+    obtain ⟨hcc, hcet, hcef⟩ := cond_closed_iff.mp hc
+    apply cond_closed_iff.mpr
+    have .cond _ _ _ _ htc htet htef := ht
+    and_intros
+    · exact ih hcc htp htc
+    · apply closed_of_step htp.validRefs htet.validRefs hcet
+      exact (.condC _ _ _ _ _ _ hs)
+    · apply closed_of_step htp.validRefs htef.validRefs hcef
+      exact (.condC _ _ _ _ _ _ hs)
